backend/Linear.v
@@ -313,10 +313,10 @@ Definition pre_main_sig: signature:=
      sig_res := None ;
      sig_cc := cc_default |}.
 *)
-Definition pre_main (stck_sz:Z): function:=
+Definition pre_main sig (stck_sz:Z): function:=
   {| fn_sig := pre_main_sig;
      fn_stacksize := stck_sz;
-     fn_code := nil |}.
+     fn_code := (Lcall sig (inr xH) ::nil) |}.
 (* loc_arguments takes a signature, 
    It generally only needs the types of arguemtns targs.
    For RISC-V, it also takes calling conventions.
@@ -327,33 +327,32 @@ Definition pre_main_locset targs args: locset:=
               sig_cc := cc_default |} in
   build_ls_from_arguments sg args.
 Definition arg_size (args : list typ):= Z.of_nat (Datatypes.length args).
-Definition pre_main_stack targs args: stackframe:=
+Definition pre_main_stack sig sp targs args: stackframe:=
   Stackframe
-    (pre_main (arg_size targs))
-    Vundef                     (* no stack pointere for pre_main *)
+    (pre_main sig 0 (*arg_size targs*))
+    (Vptr sp Ptrofs.zero)       (* no stack pointere for pre_main *)
     (pre_main_locset targs args) (* empty environment in pre_main *)
-    nil.                       (* No continuation in pre_main *)
+    nil.                         (* No continuation in pre_main *)
 
-Definition pre_main_staklist sig args:=
-  (pre_main_stack sig args)::nil.
-Definition has_pre_main (cs:list stackframe):= (0 < length cs)%nat.
+Definition pre_main_staklist sp sig targs args:=
+  (pre_main_stack sp sig targs args)::nil.
 
 
 
 Inductive entry_point (p: program): mem -> state -> val -> list val -> Prop :=
-  | entry_point_intro: forall fb f m0 m1 stk args targs,
+  | entry_point_intro: forall fb f m0 m1 sp args targs,
       let ge := Genv.globalenv p in
       Mem.mem_wd m0 ->
       globals_not_fresh ge m0 ->
       Genv.find_funct_ptr ge fb = Some (Internal f) ->
       Val.has_type_list args (sig_args (funsig (Internal f))) ->
       (* Allocate a stackframe, to pass arguments in the stack*)
-      Mem.alloc m0 0 0 = (m1, stk) ->
+      Mem.alloc m0 0 0 = (m1, sp) ->
       targs = sig_args (fn_sig f) ->
       Val.has_type_list args targs ->
       Mem.arg_well_formed args m0 ->
       let ls := LTL.build_ls_from_arguments (funsig (Internal f)) args in
-      entry_point p m0 (Callstate (pre_main_staklist targs args)
+      entry_point p m0 (Callstate (pre_main_staklist (fn_sig f) sp targs args)
                                   (Internal f) ls m1)
                   (Vptr fb Ptrofs.zero) args.
 
